

Normal Form

Theory, Examples, and Proofs

Sara Sorahi

Introduction to the Theory of Computation

Normal Forms: Basic Idea

A **normal form** is a restricted, standardized way of writing mathematical objects (formulas, grammars, rules) *without changing their meaning*.

Key principle:

Expressive Power is Preserved

Only the *syntax* is restricted — not what can be expressed.

Why Do We Use Normal Forms?

Normal forms are useful because they:

- ▶ simplify proofs
- ▶ enable algorithms
- ▶ make comparison easier
- ▶ provide a common standard

Many fundamental results in computation assume inputs are in a normal form.

Conjunctive Normal Form (CNF)

A Boolean formula is in **CNF** if:

- ▶ it is a conjunction (\wedge) of clauses
- ▶ each clause is a disjunction (\vee) of literals
- ▶ a literal is a variable or its negation

Example:

$$(p \vee \neg q \vee r) \wedge (\neg p \vee q)$$

Disjunctive Normal Form (DNF)

A Boolean formula is in **DNF** if:

- ▶ it is a disjunction (\vee) of terms
- ▶ each term is a conjunction (\wedge) of literals

Example:

$$(p \wedge q) \vee (\neg p \wedge r)$$

Normal Forms for Grammars

In formal language theory, grammars are often converted into restricted formats called **grammar normal forms**.

These transformations:

- ▶ do not change the generated language
- ▶ simplify proofs and parsing algorithms

Chomsky Normal Form (CNF)

A context-free grammar is in **Chomsky Normal Form** if all rules are of the form:

$$A \rightarrow BC \quad \text{or} \quad A \rightarrow a$$

(with a limited exception for ϵ).

The restricted rule shapes enable efficient parsing algorithms (e.g. CYK).

Normal Forms: A Unifying Tool

Across logic and language theory, normal forms share:

- ▶ equivalence to unrestricted representations
- ▶ restricted syntax
- ▶ algorithmic usefulness

Normal forms balance **expressiveness** and **computability**.

Example: Converting to CNF (Step 1)

Convert the formula to CNF:

$$\varphi = (p \rightarrow q) \wedge (r \rightarrow (p \vee s)).$$

Step 1: Eliminate implications using

$$(a \rightarrow b) \equiv (\neg a \vee b).$$

So,

$$\varphi \equiv (\neg p \vee q) \wedge (\neg r \vee (p \vee s)).$$

Example: Converting to CNF (Already Done!)

We obtained:

$$(\neg p \vee q) \wedge (\neg r \vee (p \vee s)).$$

This is already in CNF:

- ▶ a conjunction (\wedge) of clauses
- ▶ each clause is a disjunction (\vee) of literals

Example: Distribution to Reach CNF

Convert to CNF:

$$\psi = (p \vee (q \wedge r)).$$

Use distribution:

$$x \vee (y \wedge z) \equiv (x \vee y) \wedge (x \vee z).$$

So,

$$\psi \equiv (p \vee q) \wedge (p \vee r).$$

Example: A Slightly Longer CNF Conversion

Convert to CNF:

$$\theta = (p \rightarrow (q \wedge r)).$$

Step 1: remove implication

$$\theta \equiv (\neg p \vee (q \wedge r)).$$

Step 2: distribute

$$\neg p \vee (q \wedge r) \equiv (\neg p \vee q) \wedge (\neg p \vee r).$$

Proof Idea: Every Formula Has an Equivalent CNF

Claim. Every Boolean formula is equivalent to a CNF formula.

Proof strategy (constructive):

1. Eliminate \rightarrow and \leftrightarrow using equivalences.
2. Push negations inward using De Morgan + double negation:

$$\neg(a \wedge b) \equiv (\neg a \vee \neg b), \quad \neg(a \vee b) \equiv (\neg a \wedge \neg b).$$

3. Distribute \vee over \wedge until you obtain an AND of ORs.

Each step preserves equivalence, so the final CNF is equivalent to the original.

Note: Size Blow-up

CNF conversion by distribution can cause exponential growth.

Example pattern:

$$(x_1 \wedge y_1) \vee (x_2 \wedge y_2) \vee \cdots \vee (x_n \wedge y_n)$$

Distributing fully produces many clauses (can be exponential in n).

Example CFG (Not in Chomsky Normal Form)

Consider the grammar G generating $L = \{a^n b^n : n \geq 0\}$:

$$S \rightarrow aSb \mid \epsilon.$$

This is context-free, but not in CNF because:

- ▶ $S \rightarrow aSb$ has 3 symbols on the right
- ▶ $S \rightarrow \epsilon$ is an ϵ -rule

Step: Replace Terminals in Long Rules

Goal: make rules look like $A \rightarrow BC$ or $A \rightarrow a$.

Introduce new variables for terminals:

$$A \rightarrow a, \quad B \rightarrow b.$$

Rewrite:

$$S \rightarrow ASB \mid \epsilon.$$

Now terminals are isolated, but the right-hand side is still too long.

Step: Binarize Long Right-Hand Sides

We want to eliminate length-3 productions like:

$$S \rightarrow ASB.$$

Introduce a new variable C :

$$C \rightarrow SB.$$

Then replace the old rule by:

$$S \rightarrow AC \mid \epsilon, \quad C \rightarrow SB.$$

Now the non- ϵ rules are of the form $A \rightarrow BC$.

Handling the ϵ -Rule Carefully

Chomsky Normal Form allows ϵ only via:

$$S \rightarrow \epsilon$$

and only if $\epsilon \in L(G)$.

In our language $a^n b^n$, ϵ is generated (when $n = 0$), so keeping $S \rightarrow \epsilon$ is acceptable under the standard CNF convention.

Theorem: Every CFG Has an Equivalent CNF Grammar

Theorem. For every context-free grammar G , there exists a grammar G' in Chomsky Normal Form such that:

$$L(G') = L(G)$$

(or $L(G') = L(G) \setminus \{\epsilon\}$, with a standard fix if needed).

Meaning: CNF is a restriction on rule *shape*, not on expressive power.

Proof Sketch (1): Cleaning Steps

Start from any CFG G .

Apply standard equivalence-preserving transformations:

1. Remove useless symbols (non-generating / unreachable variables).
2. Eliminate ϵ -productions (except possibly $S \rightarrow \epsilon$).
3. Eliminate unit productions ($A \rightarrow B$).

Each step produces a new grammar generating the same language (with the usual ϵ caveat).

Proof Sketch (2): Put Rules Into CNF Shape

After cleaning, remaining rules have the form:

$$A \rightarrow X_1 X_2 \cdots X_k \quad (k \geq 1),$$

where each X_i is a terminal or variable.

Two final transformations:

1. **Isolate terminals:** if a terminal appears in a long RHS, replace it by a new variable (e.g., $T_a \rightarrow a$).
2. **Binarize:** replace $A \rightarrow X_1 X_2 \cdots X_k$ ($k \geq 3$) by introducing new variables so that all rules become binary.

Result: only $A \rightarrow BC$ and $A \rightarrow a$ remain (plus optional $S \rightarrow \epsilon$).

Why the Transformations Preserve the Language

Key invariant: Every new variable introduced is a “name” for a substring pattern.

Examples:

- ▶ Terminal isolation: $T_a \rightarrow a$ ensures T_a derives exactly a .
- ▶ Binarization: if $C \rightarrow X_2 \cdots X_k$, then $A \rightarrow X_1 C$ derives exactly what $A \rightarrow X_1 \cdots X_k$ derived before.

Thus, derivations in G correspond to derivations in G' and vice versa.

Proof Pattern: Equivalence via Mutual Simulation

To prove $L(G) = L(G')$, use two directions:

$$L(G) \subseteq L(G') \quad \text{and} \quad L(G') \subseteq L(G).$$

Method:

- ▶ Show how to convert any derivation in G into a derivation in G' .
- ▶ Show how to convert any derivation in G' into a derivation in G .

This is the standard “simulation” proof style for normal-form theorems.

Target Language: Simple Arithmetic Expressions

We start with a standard expression grammar (with precedence):

$$E \rightarrow E + T \mid T$$

$$T \rightarrow T * F \mid F$$

$$F \rightarrow (E) \mid id$$

Goal: Convert to **Chomsky Normal Form** (CNF):

$$A \rightarrow BC \quad \text{or} \quad A \rightarrow a$$

(and optionally $S \rightarrow \epsilon$ if needed).

Step 0: Add a New Start Symbol

Introduce a fresh start symbol S :

$$S \rightarrow E$$

This helps when removing ϵ -rules or unit productions later, and guarantees the start symbol never appears on a RHS in the final grammar.

Step 1: Remove Unit Productions

Unit productions are rules like $A \rightarrow B$. Here we have:

$$S \rightarrow E, \quad E \rightarrow T, \quad T \rightarrow F$$

Eliminate them by “copying” non-unit rules upward:

- ▶ Since $E \Rightarrow T$, add $E \rightarrow T * F \mid (E) \mid id$
- ▶ Since $T \Rightarrow F$, add $T \rightarrow (E) \mid id$
- ▶ Since $S \Rightarrow E$, let S inherit all E rules

Then delete unit productions.

Grammar After Unit-Removal (Readable Form)

After removing unit rules, we can use:

$$S \rightarrow E + T \mid T * F \mid (E) \mid id \mid T \mid F$$

$$E \rightarrow E + T \mid T * F \mid (E) \mid id \mid F$$

$$T \rightarrow T * F \mid (E) \mid id$$

$$F \rightarrow (E) \mid id$$

We can simplify: many rules are redundant, but redundancy is OK. Next we enforce CNF *shape*.

Step 2: Isolate Terminals

CNF does not allow terminals mixed inside long RHSs like:

$$E \rightarrow E + T, \quad F \rightarrow (E)$$

Introduce variables for terminals:

$$P \rightarrow +, \quad M \rightarrow *, \quad L \rightarrow (, \quad R \rightarrow)$$

Now rewrite:

$$E \rightarrow EPT, \quad T \rightarrow TMF, \quad F \rightarrow LER \mid id$$

Step 3: Binarize Long Right-Hand Sides

We must eliminate length ≥ 3 RHSs:

$$E \rightarrow EPT, \quad F \rightarrow LER$$

Introduce new variables to make everything binary:

$$X \rightarrow PT$$

$$E \rightarrow EX$$

$$Y \rightarrow ER$$

$$F \rightarrow LY$$

Now all nonterminal rules are of the form $A \rightarrow BC$.

Final CNF Grammar (One Clean Version)

A CNF grammar generating the same expression language:

$$S \rightarrow EX \mid TM \mid LY \mid id$$

$$E \rightarrow EX \mid TM \mid LY \mid id$$

$$T \rightarrow TM \mid LY \mid id$$

$$F \rightarrow LY \mid id$$

$$X \rightarrow PT$$

$$M \rightarrow MF$$

$$Y \rightarrow ER$$

$$P \rightarrow +, \quad M_t \rightarrow *, \quad L \rightarrow (, \quad R \rightarrow)$$

Notes:

- All rules are $A \rightarrow BC$ or $A \rightarrow a$.

Why This Works (Derivation Correspondence)

Claim: Every derivation step in the original grammar can be simulated.

Examples:

- ▶ Original: $E \Rightarrow E + T$ becomes

$$E \Rightarrow EX \Rightarrow EPT \Rightarrow E + T$$

(since $P \rightarrow +$).

- ▶ Original: $F \Rightarrow (E)$ becomes

$$F \Rightarrow LY \Rightarrow LER \Rightarrow (E)$$

New variables are just “helpers” that preserve the same strings.

SAT and CNF: The Core Connection

SAT asks: given a Boolean formula φ , is there an assignment that makes φ true?

In practice and in theory, formulas are often converted to **CNF**:

$$\varphi = C_1 \wedge C_2 \wedge \cdots \wedge C_m$$

where each clause C_i is an OR of literals. This is the standard input format for SAT solvers.

3SAT: A Restricted Normal Form Problem

3SAT is SAT where every clause has exactly 3 literals:

$$(x \vee y \vee z) \wedge (\neg x \vee y \vee w) \wedge \dots$$

3SAT is a **normal-form restriction**:

- ▶ fewer allowed shapes (only 3-literal clauses)
- ▶ but still captures the full computational difficulty of SAT

Theorem: SAT is in NP

Claim. $\text{SAT} \in \text{NP}$.

Proof sketch. A certificate is a truth assignment to the variables. Given an assignment, we can evaluate φ in time polynomial in $|\varphi|$ (by computing each gate/clause once). So SAT has polynomial-time verification.

Theorem: 3SAT is NP-Complete (What It Means)

Theorem. 3SAT is NP-complete.

Two parts:

- ▶ (**Membership**) $3SAT \in NP$ (same verification idea).
- ▶ (**Hardness**) Every language in NP reduces to 3SAT in polynomial time.

So 3SAT is a canonical “hardest” problem in NP.

Cook–Levin (Big Picture Proof Sketch)

Cook–Levin Theorem: SAT is NP-complete.

Idea: Encode a polynomial-time NTM computation as a Boolean formula.

- ▶ Variables represent symbols/states at positions in a computation tableau.
- ▶ Clauses enforce:
 - ▶ valid start configuration
 - ▶ valid transitions (local consistency)
 - ▶ an accepting configuration occurs

The formula is satisfiable *iff* the machine accepts the input.

From SAT to 3SAT (Normal-Form Reduction)

Claim. $\text{SAT} \leq_p \text{3SAT}$.

Proof sketch: Convert an arbitrary CNF clause to 3-literal clauses.

- ▶ If a clause has 1 or 2 literals, pad by repeating literals:

$$(x) \equiv (x \vee x \vee x), \quad (x \vee y) \equiv (x \vee y \vee y)$$

- ▶ If a clause has $k > 3$ literals:

$$(l_1 \vee l_2 \vee \cdots \vee l_k)$$

introduce new variables y_1, \dots, y_{k-3} and replace by:

$$(l_1 \vee l_2 \vee y_1) \wedge (\neg y_1 \vee l_3 \vee y_2) \wedge \cdots \wedge (\neg y_{k-3} \vee l_{k-1} \vee l_k)$$

Satisfiability is preserved, and the size grows only linearly.

Takeaway: Normal Forms Power NP-Completeness

Normal forms are not just “pretty formatting”: they enable clean reductions and standard problem statements.

Examples:

- ▶ CNF makes SAT solver inputs uniform.
- ▶ 3CNF makes hardness proofs modular and reusable.
- ▶ Tableau-style encodings rely on strict local constraints (a kind of normal form).